SkLean/Proof.lean
@@ -3,4 +3,9 @@ import SkLean.EvalTactic
 
 example : beta_eq SKM[((K x) y)] x := by
   eval_to x
-  
+
+example : beta_eq SKM[(((S K) K) K)] SKM[K] := by
+  eval_to SKM[K]
+
+example : beta_eq SKM[(M (((S K) K) K))] SKM[(M K)] := by
+  eval_to SKM[(M K)]
